Rope/Pred.lean
@@ -13,15 +13,6 @@ namespace Pred
 
 -- TODO This should almost certainly be mutually inductive with Row and Pred
 -- This should (maybe?) bundle evidence eventually
-inductive Pred : Type where
-  | Contain (x: Row) (y: Row) : Pred
-    -- Garrett-style 3-place concatenation predicate
-    -- x + y ~ z
-  | Combine (x: Row) (y: Row) (z: Row) : Pred
-  -- Eq can defined in terms of Combine, at the cost of always introducing another type variable
-  -- | Eq (x: Row) (y: Row) : Pred
-  -- May want separate disjointness or lack constraints.
-  | TyEq (t1 t2 : Ty) : Pred
 
 inductive Entail : Pred -> Pred -> Prop where
   -- | Contain : (x ≤ y) -> Entail x y
